code/ecdsap256/Hacl.Impl.P256.MixedPointAdd.fst
@@ -1,0 +1,81 @@
+module Hacl.Impl.P256.MixedPointAdd
+
+open FStar.HyperStack.All
+open FStar.HyperStack
+module ST = FStar.HyperStack.ST
+
+open Lib.IntTypes
+open Lib.Buffer
+
+open Spec.P256.Definitions
+open Spec.P256.Lemmas
+
+open FStar.Math
+open FStar.Math.Lemmas
+open FStar.Mul
+
+open Hacl.Impl.P256.LowLevel
+open Hacl.Impl.P256.PointAdd
+
+
+
+inline_for_extraction
+type pointAffine = lbuffer uint64 (size 8)
+
+val pointAffineIsNotZero: p: pointAffine -> Stack uint64
+  (requires fun h -> live h p)
+  (ensures fun h0 r h1 -> modifies0 h0 h1 /\ 
+    (
+      let x = gsub p (size 0) (size 4) in 
+      let y = gsub p (size 4) (size 4) in 
+      if as_nat h0 x = 0 || as_nat h0 y = 0 then uint_v r = pow2 64 - 1 else uint_v r == 0))
+  
+
+let pointAffineIsNotZero p = 
+  let x = sub p (size 0) (size 4) in 
+  let y = sub p (size 4) (size 4) in 
+  let xZero = isZero_uint64_CT x in 
+  let yZero = isZero_uint64_CT y in 
+  logor_lemma xZero yZero;
+  logor xZero yZero
+
+
+val copy_point_conditional: out: point -> p: pointAffine -> maskPoint: point -> Stack unit 
+  (requires fun h -> live h out /\ live h p /\ live h maskPoint /\ 
+    LowStar.Monotonic.Buffer.all_disjoint [loc p |+| loc out |+| loc maskPoint] /\
+    (
+      let xOut = as_nat h (gsub out (size 0) (size 4)) in 
+      let yOut = as_nat h (gsub out (size 4) (size 4)) in 
+      let zOut = as_nat h (gsub out (size 8) (size 4)) in 
+      xOut < prime256 /\ yOut < prime256 /\ zOut < prime256 /\
+      as_nat h (gsub p (size 0) (size 4)) < prime256 /\ 
+      as_nat h (gsub p (size 4) (size 4)) < prime256
+    )
+  )
+  (ensures fun h0 _ h1 -> True) 
+
+let copy_point_conditional out p maskPoint = 
+  let z = sub maskPoint (size 8) (size 4) in 
+  let mask = isZero_uint64_CT z in 
+
+  let xOut = sub out (size 0) (size 4) in 
+  let yOut = sub out (size 4) (size 4) in 
+  let zOut = sub out (size 8) (size 4) in 
+
+  let p_x = sub p (size 0) (size 4) in 
+  let p_y = sub p (size 4) (size 4) in 
+
+  copy_conditional xOut p_x mask;
+  copy_conditional yOut p_y mask;
+  (* 1 should be in Domaine*)
+  copy_conditional zOut (u64 1) mask
+
+
+(* we except that we already know the q point *)
+val pointAddMixed: result: point -> p: point -> q: pointAffine -> Stack unit 
+  (requires fun h -> live h result /\ live h p /\ live h q)
+  (ensures fun h0 _ h1 -> True)
+
+
+let pointAddMixed result p q = 
+  copy_point_conditional result q p
